ironfleet/src/Dafny/Distributed/Impl/WS/PacketParsing.i.dfy
@@ -11,15 +11,29 @@ import opened Common__NodeIdentity_i
 import opened WS__Environment_i
 import opened WS__Host_i
 
+function method EndPoint_grammar() : G { GUint64 }
+
+function method parse_EndPoint(val:V) : EndPoint
+    requires ValInGrammar(val, EndPoint_grammar());
+    ensures  EndPointIsAbstractable(parse_EndPoint(val));
+{
+    if val.u <= 0xffffffffffff then
+        ConvertUint64ToEndPoint(val.u)
+    else
+        EndPoint([0,0,0,0], 0)
+}
+
+
 /*
 ////////////////////////////////////////////////////////////////////
 //    Grammars for the basic types
 ////////////////////////////////////////////////////////////////////
+
+
 function method OptionalValue_grammar() : G { GTaggedUnion([Value_grammar(), GTuple([])]) }
 function method KeyPlus_grammar() : G { GTaggedUnion([Key_grammar(), GUint64]) }
 function method KeyRange_grammar() : G { GTuple([KeyPlus_grammar(), KeyPlus_grammar()]) }
 function method Hashtable_grammar() : G { GArray(GTuple([Key_grammar(), Value_grammar()])) }
-function method EndPoint_grammar() : G { GUint64 }
 
 ////////////////////////////////////////////////////////////////////
 //    Grammars for the SHT messages 
@@ -77,63 +91,7 @@ lemma lemma_CMessageGrammarValid()
 //    Parsing
 ////////////////////////////////////////////////////////////////////
 
-function method parse_OptionalValue(val:V) : OptionalValue
-    requires ValInGrammar(val, OptionalValue_grammar());
-{
-    if val.c == 0 then
-        ValuePresent(parse_Value(val.val))
-    else 
-        ValueAbsent()
-}
 
-function method parse_KeyPlus(val:V) : KeyPlus
-    requires ValInGrammar(val, KeyPlus_grammar());
-{
-    if val.c == 0 then
-        KeyPlus(parse_Key(val.val))
-    else if val.c == 1 then
-        if val.val.u == 0 then
-            KeyZero()
-        else 
-            KeyInf()
-    else
-        assert false;       // Should never get here
-        KeyInf()
-}
-
-function method parse_KeyRange(val:V) : KeyRange
-    requires ValInGrammar(val, KeyRange_grammar());
-{
-    KeyRange(parse_KeyPlus(val.t[0]), parse_KeyPlus(val.t[1]))
-}
-
-function method parse_Hashtable(val:V) : Hashtable 
-    requires ValInGrammar(val, Hashtable_grammar());
-    ensures  |parse_Hashtable(val)| <= |val.a|;
-    ensures  ValidVal(val) ==> HashtableIs64Bit(parse_Hashtable(val));
-    decreases |val.a|;
-{
-    if |val.a| == 0 then
-        map []
-    else 
-        var tuple := val.a[0];
-        assert ValInGrammar(tuple, Hashtable_grammar().elt);        // OBSERVE: Still needed despite fuel boost.  Odd.
-        var key := parse_Key(tuple.t[0]);
-        var value := parse_Value(tuple.t[1]);
-        var others := parse_Hashtable(VArray(val.a[1..]));
-        var m := others[key := value];
-        m
-}
-
-function method parse_EndPoint(val:V) : EndPoint
-    requires ValInGrammar(val, EndPoint_grammar());
-    ensures  EndPointIsAbstractable(parse_EndPoint(val));
-{
-    if val.u <= 0xffffffffffff then
-        ConvertUint64ToEndPoint(val.u)
-    else
-        EndPoint([0,0,0,0], 0)
-}
 
 function method parse_Message_GetRequest(val:V) : CMessage
     requires ValInGrammar(val, CMessage_GetRequest_grammar());
@@ -211,17 +169,18 @@ function method {:fuel ValidVal,2} parse_CSingleMessage(val:V) : CSingleMessage
     else
         CAck(val.val.u)
 }
+*/
 
-function SHTDemarshallData(data:seq<byte>) : CSingleMessage
+function SHTDemarshallData(data:seq<byte>) : CMessage
 {
-    if Demarshallable(data, CSingleMessage_grammar()) then
+    if Demarshallable(data, CMessage_grammar()) then
     var val := DemarshallFunc(data, CSingleMessage_grammar());
-    parse_CSingleMessage(val)
+    parse_CMessage(val)
     else
         CInvalidMessage()
 }
 
-method SHTDemarshallDataMethod(data:array<byte>) returns (msg:CSingleMessage)
+method WSDemarshallDataMethod(data:array<byte>) returns (msg:CMessage)
     requires data != null;
     requires data.Length < 0x1_0000_0000_0000_0000;
     ensures  CSingleMessageIs64Bit(msg); 
@@ -241,23 +200,6 @@ method SHTDemarshallDataMethod(data:array<byte>) returns (msg:CSingleMessage)
     }
 }
 
-///////////////////////////////////////////////////////////////////
-//    64-bit Limits
-////////////////////////////////////////////////////////////////////
-
-predicate HashtableIs64Bit(h:Hashtable) { |h| < 0x1_0000_0000_0000_0000 }
-
-predicate CMessageIs64Bit(m:CMessage)
-{
-    m.CDelegate? ==> HashtableIs64Bit(m.h)
-}
-
-predicate CSingleMessageIs64Bit(msg:CSingleMessage) 
-{
-    msg.CSingleMessage? ==> CMessageIs64Bit(msg.m)
-}
-*/
-
 ////////////////////////////////////////////////////////////////////
 //    Marshalling 
 ////////////////////////////////////////////////////////////////////
@@ -267,144 +209,24 @@ predicate CMessageMarshallable(msg:CMessage)
     true
 }
 
+
 /*
-method IsValidKeyPlus(kp:KeyPlus) returns (b:bool)
-    ensures b == ValidKeyPlus(kp);
-{
-    if kp.KeyZero? || kp.KeyInf? {
-        b := true;
-    } else {
-        b := IsKeyValid(kp.k);
-    }
-}
-
-method IsValidKeyRange(kr:KeyRange) returns (b:bool)
-    ensures b == ValidKeyRange(kr);
-{
-    b := IsValidKeyPlus(kr.klo);
-    if b {
-        b := IsValidKeyPlus(kr.khi);
-    }
-}
-
-method IsEmptyKeyRange(kr:KeyRange) returns (b:bool)
-    ensures b == EmptyKeyRange(kr);
-{
-    if kr.khi == kr.klo {
-        b := true;
-    } else {
-        match kr.khi {
-            case KeyZero => b := true;
-            case KeyInf  => b := false;
-            case KeyPlus(k) =>
-                match kr.klo {
-                    case KeyZero => b := false;
-                    case KeyInf  => b := true;
-                    case KeyPlus(k') => b := IsKeyLt(k, k');
-                }
-        }
-    }
-}
-
-method IsValidHashtable(h:Hashtable) returns (b:bool)
-    requires HashtableIs64Bit(h);
-    ensures  b == ValidHashtable(h);
-{
-    b := uint64(|h|) < 62;  // max_hashtable_size
-
-    if !b { return; }
-
-    var keys := domain(h);
-    lemma_MapSizeIsDomainSize(keys, h);
-
-    while uint64(|keys|) > 0
-        invariant |keys| < max_hashtable_size();
-        invariant forall k :: k in keys ==> k in h;
-        invariant forall k :: k in h ==> k in keys || (ValidKey(k) && ValidValue(h[k]));
-        decreases |keys|;
-    {
-        var k :| k in keys;
-        keys := keys - {k};
-        b := IsKeyValid(k);
-        if !b {
-            return;
-        }
-        b := IsValueValid(h[k]);
-        if !b {
-            return;
-        }
-    }
-}
-
 method IsMessageMarshallable(msg:CMessage) returns (b:bool)
     requires CMessageIs64Bit(msg);
     requires CMessageIsAbstractable(msg);
     ensures  b == MessageMarshallable(msg);
 {
-    match msg 
-        case CGetRequest(k) => b := IsKeyValid(k);
-        case CSetRequest(k, v) =>
-            b := IsKeyValid(k);
-            if b && v.ValuePresent? {
-                b := IsValueValid(v.v);
-            }
-        case CReply(k, v) => 
-            b := IsKeyValid(k);
-            if b && v.ValuePresent? {
-                b := IsValueValid(v.v);
-            }
-        case CRedirect(k, id) => 
-            b := IsKeyValid(k);
-            b := b && (uint64(|id.addr|) == 4 && 0 <= id.port <= 65535);
-        case CShard(kr, id) => 
-            b := IsValidKeyRange(kr);
-            b := b && (uint64(|id.addr|) == 4 && 0 <= id.port <= 65535);
-            if b {
-                b := IsEmptyKeyRange(kr);
-                b := !b;
-            }
-        case CDelegate(kr, h) => 
-            b := IsValidKeyRange(kr);
-            if b {
-                b := IsValidHashtable(h);
-                if b {
-                    b := IsEmptyKeyRange(kr);
-                    b := !b;
-                }
-            }
-}
-
-method IsCSingleMessageMarshallable(msg:CSingleMessage) returns (b:bool)
-    requires CSingleMessageIsAbstractable(msg);
-    requires CSingleMessageIs64Bit(msg);
-    ensures  b == CSingleMessageMarshallable(msg);
-{
-    if msg.CAck? {
-        b := true;
-    } else if msg.CInvalidMessage? {
-        b := false;
-    } else {
-        assert msg.CSingleMessage?;
-
-        if !(uint64(|msg.dst.addr|) == 4 && 0 <= msg.dst.port <= 65535) {
-            b := false;
-            return;
-        }
-
-        b := IsMessageMarshallable(msg.m);
-    }
-
-}
-
+    b := true;
+}*/
 
 function CMessageIsValid(msg:CMessage) : bool
 {
-    MessageMarshallable(msg)
+    CMessageMarshallable(msg)
 }
 
 predicate CPacketIsMarshallable(cp:CPacket)
 {
-    EndPointIsAbstractable(cp.src) && EndPointIsAbstractable(cp.dst) && CSingleMessageMarshallable(cp.msg) && (cp.msg.CSingleMessage? && cp.msg.m.CShard? ==> cp.msg.m.recipient != cp.dst)
+    EndPointIsAbstractable(cp.src) && EndPointIsAbstractable(cp.dst) && CMessageMarshallable(cp.msg)
 }
 
 predicate CPacketsIsMarshallable(cps:set<CPacket>)
@@ -412,145 +234,6 @@ predicate CPacketsIsMarshallable(cps:set<CPacket>)
     forall cp :: cp in cps ==> CPacketIsMarshallable(cp)
 }
 
-
-method MarshallOptionalValue(c:OptionalValue) returns (val:V)
-    requires ValidOptionalValue(c);
-    ensures  ValInGrammar(val, OptionalValue_grammar());
-    ensures  ValidVal(val);
-    ensures  parse_OptionalValue(val) == c;
-    ensures  0 <= SizeOfV(val) < 16 + max_val_len();
-{
-    if c.ValuePresent? {
-        var v := MarshallValue(c.v);
-        val := VCase(0, v);
-    } else {
-        reveal_SeqSum();
-        val := VCase(1, VTuple([]));
-    }
-}
-
-method MarshallKeyPlus(c:KeyPlus) returns (val:V)
-    requires ValidKeyPlus(c);
-    ensures  ValInGrammar(val, KeyPlus_grammar());
-    ensures  ValidVal(val);
-    ensures  parse_KeyPlus(val) == c;
-    ensures  0 <= SizeOfV(val) < 16 + max_key_len();
-{
-    if c.KeyPlus? {
-        var key := MarshallKey(c.k);
-        val := VCase(0, key);
-    } else if c.KeyZero? {
-        val := VCase(1, VUint64(0));
-    } else {
-        val := VCase(1, VUint64(42));
-    }
-}
-
-method MarshallKeyRange(c:KeyRange) returns (val:V)
-    requires ValidKeyRange(c);
-    ensures  ValInGrammar(val, KeyRange_grammar());
-    ensures  ValidVal(val);
-    ensures  parse_KeyRange(val) == c;
-    ensures  0 <= SizeOfV(val) < (16 + max_key_len()) + (16 + max_key_len());
-{
-    var klo := MarshallKeyPlus(c.klo);
-    var khi := MarshallKeyPlus(c.khi);
-    val := VTuple([klo, khi]);
-    lemma_SeqSum_2(val);
-}
-
-// TODO: Refactor this and Paxos' version to put them in a common location
-lemma lemma_SeqSum_2(val:V)
-    requires val.VTuple?;
-    requires |val.t| == 2;
-    ensures  SizeOfV(val) == SizeOfV(val.t[0]) + SizeOfV(val.t[1]);
-{
-    calc {
-        SeqSum(val.t);
-            { reveal_SeqSum(); }
-        SizeOfV(val.t[0]) + SeqSum(val.t[1..]);
-            { reveal_SeqSum(); }
-        SizeOfV(val.t[0]) + SizeOfV(val.t[1]) + SeqSum(val.t[2..]);
-            { assert val.t[2..] == []; }        // OBSERVE
-        SizeOfV(val.t[0]) + SizeOfV(val.t[1]) + SeqSum([]);
-            { reveal_SeqSum(); }
-        SizeOfV(val.t[0]) + SizeOfV(val.t[1]);
-    }
-}
-
-lemma lemma_SeqSum_3(val:V)
-    requires val.VTuple?;
-    requires |val.t| == 3;
-    ensures  SizeOfV(val) == SizeOfV(val.t[0]) + SizeOfV(val.t[1]) + SizeOfV(val.t[2]);
-{
-    calc {
-        SeqSum(val.t);
-            { reveal_SeqSum(); }
-        SizeOfV(val.t[0]) + SeqSum(val.t[1..]);
-            { reveal_SeqSum(); }
-        SizeOfV(val.t[0]) + SizeOfV(val.t[1]) + SeqSum(val.t[2..]);
-            { reveal_SeqSum(); }
-        SizeOfV(val.t[0]) + SizeOfV(val.t[1]) + SizeOfV(val.t[2]) + SeqSum(val.t[3..]);
-            { assert val.t[3..] == []; }        // OBSERVE
-        SizeOfV(val.t[0]) + SizeOfV(val.t[1]) + SizeOfV(val.t[2]) + SeqSum([]);
-            { reveal_SeqSum(); }
-        SizeOfV(val.t[0]) + SizeOfV(val.t[1]) + SizeOfV(val.t[2]);
-    }
-
-}
-
-method MarshallHashtable(c:Hashtable) returns (val:V)
-    requires ValidHashtable(c);
-    ensures  ValInGrammar(val, Hashtable_grammar());
-    ensures  ValidVal(val);
-    ensures  parse_Hashtable(val) == c;
-    ensures  |c| == |val.a|;
-    ensures SeqSum(val.a) <= |c| * ((8 + max_key_len()) + (8 + max_val_len()));
-{
-    if |c| == 0 {
-        val := VArray([]);
-        reveal_SeqSum();
-    } else {
-        lemma_non_empty_map_has_elements(c);
-        var key := 0;
-        key :| key in c;
-        var marshalled_key := MarshallKey(key);
-        var marshalled_value := MarshallValue(c[key]);
-        var remainder := RemoveElt(c, key);
-        var marshalled_remainder := MarshallHashtable(remainder);
-        assert parse_Hashtable(marshalled_remainder) == remainder;
-        val := VArray([VTuple([marshalled_key, marshalled_value])] + marshalled_remainder.a);
-
-        // OBSERVE (everything below; not sure which bit is critical to proving the final ensures)
-        ghost var tuple := val.a[0];
-        ghost var rest := val.a[1..];
-        ghost var key' := parse_Key(tuple.t[0]);
-        ghost var value' := parse_Value(tuple.t[1]);
-        ghost var others' := parse_Hashtable(VArray(val.a[1..]));
-        ghost var m' := others'[key' := value'];
-        assert key' == key;
-        assert value' == c[key];
-        assert others' == remainder;
-        assert m' == c;
-
-        // Prove the SeqSum ensures
-        calc {
-            SeqSum(val.a);
-                { reveal_SeqSum(); }
-            SizeOfV(val.a[0]) + SeqSum(val.a[1..]);
-            <=  
-            SizeOfV(val.a[0]) + |remainder| * ((8 + max_key_len()) + (8 + max_val_len()));
-                { lemma_SeqSum_2(val.a[0]); }
-            SizeOfV(val.a[0].t[0]) + SizeOfV(val.a[0].t[1]) + |remainder| * ((8 + max_key_len()) + (8 + max_val_len()));
-            <   //{ lemma_Vote_Val_Valid(c[op], val.a[0].t[1]); lemma_Vote_bound(c[op], val.a[0].t[1]); }
-            ((8 + max_key_len()) + (8 + max_val_len())) + |remainder| * ((8 + max_key_len()) + (8 + max_val_len()));
-            1*((8 + max_key_len()) + (8 + max_val_len())) + |remainder| * ((8 + max_key_len()) + (8 + max_val_len()));
-                { lemma_mul_is_distributive(((8 + max_key_len()) + (8 + max_val_len())), 1, |remainder|); }
-            (1+|remainder|) * ((8 + max_key_len()) + (8 + max_val_len()));
-            |c| * ((8 + max_key_len()) + (8 + max_val_len()));
-        }
-    }
-}
 
 method MarshallEndPoint(c:EndPoint) returns (val:V)
     requires EndPointIsAbstractable(c);
@@ -563,28 +246,14 @@ method MarshallEndPoint(c:EndPoint) returns (val:V)
 }
 
 method MarshallMessage_GetRequest(c:CMessage) returns (val:V)
-    requires MessageMarshallable(c);
+    requires CMessageMarshallable(c);
     requires c.CGetRequest?;
     ensures  ValInGrammar(val, CMessage_GetRequest_grammar());
     ensures  ValidVal(val);
-    ensures  parse_Message_GetRequest(val) == c;
+    ensures  parse_CMessage_GetRequest(val) == c;
     ensures  0 <= SizeOfV(val) < MaxPacketSize() - 32;
 {
     val := MarshallKey(c.k_getrequest);
-}
-
-method MarshallMessage_SetRequest(c:CMessage) returns (val:V)
-    requires MessageMarshallable(c);
-    requires c.CSetRequest?;
-    ensures  ValInGrammar(val, CMessage_SetRequest_grammar());
-    ensures  ValidVal(val);
-    ensures  parse_Message_SetRequest(val) == c;
-    ensures  0 <= SizeOfV(val) < MaxPacketSize() - 32;
-{
-    var k_setrequest := MarshallKey(c.k_setrequest);
-    var v_setrequest := MarshallOptionalValue(c.v_setrequest);
-    val := VTuple([k_setrequest, v_setrequest]);
-    lemma_SeqSum_2(val);
 }
 
 method MarshallMessage_Reply(c:CMessage) returns (val:V)
@@ -601,63 +270,6 @@ method MarshallMessage_Reply(c:CMessage) returns (val:V)
     lemma_SeqSum_2(val);
 }
 
-method MarshallMessage_Redirect(c:CMessage) returns (val:V)
-    requires MessageMarshallable(c);
-    requires c.CRedirect?;
-    ensures  ValInGrammar(val, CMessage_Redirect_grammar());
-    ensures  ValidVal(val);
-    ensures  parse_Message_Redirect(val) == c;
-    ensures  0 <= SizeOfV(val) < MaxPacketSize() - 32;
-{
-    var k_redirect := MarshallKey(c.k_redirect);
-    var ep := MarshallEndPoint(c.id);
-    val := VTuple([k_redirect, ep]);
-    lemma_SeqSum_2(val);
-}
-
-method MarshallMessage_Shard(c:CMessage) returns (val:V)
-    requires MessageMarshallable(c);
-    requires c.CShard?;
-    ensures  ValInGrammar(val, CMessage_Shard_grammar());
-    ensures  ValidVal(val);
-    ensures  parse_Message_Shard(val) == c;
-    ensures  0 <= SizeOfV(val) < MaxPacketSize() - 32;
-{
-    var k_redirect := MarshallKeyRange(c.kr);
-    var ep := MarshallEndPoint(c.recipient);
-    val := VTuple([k_redirect, ep]);
-    lemma_SeqSum_2(val);
-}
-
-method MarshallMessage_Delegate(c:CMessage) returns (val:V)
-    requires MessageMarshallable(c);
-    requires c.CDelegate?;
-    ensures  ValInGrammar(val, CMessage_Delegate_grammar());
-    ensures  ValidVal(val);
-    ensures  parse_Message_Delegate(val) == c;
-    ensures  0 <= SizeOfV(val) < MaxPacketSize() - 32;
-{
-    var range := MarshallKeyRange(c.range);
-    var h := MarshallHashtable(c.h);
-    val := VTuple([range, h]);
-
-    calc {
-        SizeOfV(val);
-            { lemma_SeqSum_2(val); }
-        SizeOfV(val.t[0]) + SizeOfV(val.t[1]);
-        < 
-        (16 + max_key_len()) + (16 + max_key_len()) + SizeOfV(val.t[1]);
-        <=
-        (16 + max_key_len()) + (16 + max_key_len()) + 8 + |c.h| * ((8 + max_key_len()) + (8 + max_val_len()));
-            { lemma_mul_is_distributive_add_forall(); } 
-        (16 + max_key_len()) + (16 + max_key_len()) + 8 + |c.h| * (8 + max_key_len()) + |c.h| * (8 + max_val_len());
-            { lemma_mul_is_distributive_add_forall(); } 
-        (16 + max_key_len()) + (16 + max_key_len()) + 8 + |c.h| * 8 + |c.h| * max_key_len() + |c.h| * 8 + |c.h| * max_val_len();
-        <
-        MaxPacketSize() - 32;
-    }
-
-}
 
 method MarshallMessage(c:CMessage) returns (val:V)
     requires MessageMarshallable(c);
@@ -669,43 +281,11 @@ method MarshallMessage(c:CMessage) returns (val:V)
     if c.CGetRequest? {
         var msg := MarshallMessage_GetRequest(c);  
         val := VCase(0, msg); 
-    } else if c.CSetRequest? {
-        var msg := MarshallMessage_SetRequest(c);  
-        val := VCase(1, msg); 
-    } else if c.CReply? {
+    } else if c.CGetResponse? {
         var msg := MarshallMessage_Reply(c);  
         val := VCase(2, msg); 
-    } else if c.CRedirect? {
-        var msg := MarshallMessage_Redirect(c);  
-        val := VCase(3, msg); 
-    } else if c.CShard? {
-        var msg := MarshallMessage_Shard(c);  
-        val := VCase(4, msg); 
-    } else if c.CDelegate? {
-        var msg := MarshallMessage_Delegate(c);  
-        val := VCase(5, msg); 
     } else {
         assert false;
-    }
-}
-
-method MarshallCSingleMessage(c:CSingleMessage) returns (val:V)
-    requires CSingleMessageMarshallable(c);
-    ensures  ValInGrammar(val, CSingleMessage_grammar());
-    ensures  ValidVal(val);
-    ensures  parse_CSingleMessage(val) == c;
-    ensures  0 <= SizeOfV(val) < MaxPacketSize();
-{
-    if c.CSingleMessage? {
-        var ep := MarshallEndPoint(c.dst);
-        var msg := MarshallMessage(c.m);
-
-        var tuple := VTuple([VUint64(c.seqno), ep, msg]);
-        lemma_SeqSum_3(tuple);
-        assert ValidVal(tuple);     // OBSERVE
-        val := VCase(0, tuple);
-    } else {
-        val := VCase(1, VUint64(c.ack_seqno));
     }
 }
 
@@ -720,17 +300,7 @@ function AbstractifyBufferToLWSPacket(src:EndPoint, dst:EndPoint, data:seq<byte>
 {
     LPacket(AbstractifyEndPointToNodeIdentity(dst),
            AbstractifyEndPointToNodeIdentity(src),
-           AbstractifyCSingleMessageToSingleMessage(SHTDemarshallData(data)))
-}
-
-predicate BufferRefinementAgreesWithMessageRefinement(msg:CSingleMessage, marshalled:seq<byte>)
-    requires CSingleMessageIsAbstractable(msg);
-    requires CSingleMessageIsAbstractable(msg);
-{
-    forall src, dst :: (EndPointIsValidIPV4(src) && EndPointIsValidIPV4(dst)) ==>
-
-            (AbstractifyBufferToLWSPacket(src, dst, marshalled)
-            == LPacket(AbstractifyEndPointToNodeIdentity(dst), AbstractifyEndPointToNodeIdentity(src), AbstractifyCSingleMessageToSingleMessage(msg)))
+           AbstractifyCMessageToMessage(WSDemarshallData(data)))
 }
 
 function AbstractifyCPacketToLWSPacket(cp:CPacket) : LWSPacket
@@ -746,7 +316,7 @@ function AbstractifyUdpPacketToLWSPacket(udp:UdpPacket) : LWSPacket
     AbstractifyBufferToLWSPacket(udp.src, udp.dst, udp.msg)
 }
 
-function AbstractifyUdpPacketToShtPacket(udp:UdpPacket) : Packet
+function AbstractifyUdpPacketToWSPacket(udp:UdpPacket) : Packet
     requires UdpPacketIsAbstractable(udp);
 {
     var lp:= AbstractifyUdpPacketToLWSPacket(udp);
@@ -759,6 +329,7 @@ predicate UdpPacketIsAbstractable(udp:UdpPacket)
     && EndPointIsValidIPV4(udp.dst)
 }
 
+/*
 predicate UdpPacketsIsAbstractable(udpps:set<UdpPacket>)
 {
     forall p :: p in udpps ==> UdpPacketIsAbstractable(p)
